

This handout includes space for every question that requires a written response. Please feel free to use it to handwrite your solutions (legibly, please). If you choose to typeset your solutions, the `README.md` for this assignment includes instructions to regenerate this handout with your typeset \LaTeX solutions.

4.a

Let $\mathbf{A} \in \mathbb{R}^{n \times d}$ with SVD $\mathbf{A} = \mathbf{U}\mathbf{D}\mathbf{V}^T$, where $\mathbf{U} \in \mathbb{R}^{n \times r}$, $\mathbf{D} \in \mathbb{R}^{r \times r}$, and $\mathbf{V}^{d \times r}$. Let $u_{ij} = (\mathbf{U})_{ij}$, $v_{ij} = (\mathbf{V})_{ij}$, and $\sigma_i = \mathbf{D}_{ii}$.

Note that

$$(\mathbf{U}\mathbf{D})_{ij} = \sum_{k=1}^r u_{ik} \delta_{kj} \sigma_j = u_{ij} \sigma_j$$

where δ_{kj} is the Kronecker delta function. From this, we get

$$(\mathbf{U}\mathbf{D}\mathbf{V}^T)_{ij} = \sum_{k=1}^r (\mathbf{U}\mathbf{D})_{ik} (\mathbf{V}^T)_{kj} = \sum_{k=1}^r \sigma_k u_{ik} v_{jk}.$$

Let \mathbf{u}_i and \mathbf{v}_i be the i th columns of \mathbf{U} and \mathbf{V} , respectively. Then kl -th entry of $\mathbf{u}_i \mathbf{v}_i^T$ is $u_{ki} v_{li}$. Hence

$$\left(\sum_{i=1}^r \sigma_i \mathbf{u}_i \mathbf{v}_i^T \right)_{kl} = \sum_{i=1}^r \sigma_i (\mathbf{u}_i \mathbf{v}_i^T)_{kl} = \sum_{i=1}^r \sigma_i u_{ki} v_{li},$$

which is precisely the expression found above for $(\mathbf{U}\mathbf{D}\mathbf{V}^T)_{kl}$.

4.b

By part (a), we know

$$\mathbf{A} = \sum_{k=1}^r \sigma_k \mathbf{u}_k \mathbf{v}_k^T.$$

Using this expression for \mathbf{A} combined with the orthonormality of the columns of \mathbf{V} , we see

$$\mathbf{A} \mathbf{v}_i = \sum_{k=1}^r \sigma_k \mathbf{u}_k \mathbf{v}_k^T \mathbf{v}_i = \sigma_i \mathbf{u}_i.$$

Thus scaling by $1/\sigma_i$ gives the desired result.

4.c

In part (a), we have already seen that row s of \mathbf{A} , denoted \mathbf{a}_s , can be written as

$$\mathbf{a}_s = \left[\sum_{i=1}^r \sigma_i u_{si} v_{1i} \quad \sum_{i=1}^r \sigma_i u_{si} v_{2i} \quad \cdots \quad \sum_{i=1}^r \sigma_i u_{si} v_{di} \right] = \sum_{i=1}^r \sigma_i u_{si} \mathbf{v}_i^T,$$

so by definition of \mathbf{A}_k , we set the all but the k largest singular values to zero and get an expression for row s of \mathbf{A}_k , denoted by \mathbf{a}_{ks} ,

$$\mathbf{a}_{ks} = \sum_{i=1}^k \sigma_i u_{si} \mathbf{v}_i^T.$$

Using the hint and the fact that the \mathbf{v}_i form an orthonormal basis for V_k , the projections onto \mathbf{v}_i are simply

$$(\mathbf{a}_s \cdot \mathbf{v}_i) \mathbf{v}_i = \sigma_i u_{si} \mathbf{v}_i,$$

so we get

$$\mathbf{a}_{ks} = \sum_{i=1}^k \sigma_i u_{si} \mathbf{v}_i^T = \sum_{i=1}^k (\mathbf{a}_s \cdot \mathbf{v}_i) \mathbf{v}_i^T$$

as desired.

4.d

Since the square root is a strictly increasing function on $[0, \infty)$, we can equivalently minimize the square of the Frobenius norm.

Suppose \mathbf{B} is a rank k matrix in $\mathbb{R}^{n \times d}$ and let \mathbf{a}_s and \mathbf{b}_s be the s th rows of \mathbf{A} and \mathbf{B} , respectively. Let a_{ij} and b_{ij} be the ij -th entries of \mathbf{A} and \mathbf{B} , respectively. Then the square of the Frobenius norm of $\mathbf{A} - \mathbf{B}$ is

$$\|\mathbf{A} - \mathbf{B}\|_F^2 = \sum_{i=1}^n \sum_{j=1}^d (a_{ij} - b_{ij})^2 = \sum_{i=1}^n \|\mathbf{a}_i - \mathbf{b}_i\|_2^2.$$

Let B be the rowspace of \mathbf{B} . The projection of \mathbf{a}_i onto B minimizes the distance between \mathbf{a}_i and any vector in B , so if we want to find a rank k matrix \mathbf{B} minimizing $\|\mathbf{A} - \mathbf{B}\|_F^2$, we can assume $\mathbf{b}_i = \text{proj}_B(\mathbf{a}_i)$. However, this sum is minimized precisely when $B = V_k$ by properties of the SVD of \mathbf{A} . By part (c), we have $\text{proj}_{V_k}(\mathbf{a}_i) = \mathbf{a}_{ki}$, the i th row of \mathbf{A}_k , so $\|\mathbf{A} - \mathbf{B}\|_F^2$ is minimized when $\mathbf{B} = \mathbf{A}_k$. (Note it is not unique if V_k does not contain the entire subspace generated by all singular vectors corresponding to the smallest singular value σ_k .)